when to keep/cast back to caller format vs when to adopt callee format?
postponing, just using string of uint8 instead of string of chars

LiveVerif/src/LiveVerifExamples/nt_uint8_string.v
@@ -25,31 +25,23 @@ Module List.
   End Lexicographic.
 End List.
 
-Module byte.
-  Definition compare(x y: byte): comparison :=
-    Z.compare (byte.unsigned x) (byte.unsigned y).
-End byte.
-
 Load LiveVerif.
 
-Definition char(c: byte): word -> mem -> Prop :=
-  uint 8 (byte.unsigned c).
-
-Definition nt_str(s: list byte)(a: word): mem -> Prop :=
-  sep (array char (len s + 1) (s ++ [| Byte.x00 |]) a)
-      (emp (~ List.In Byte.x00 s)).
+Definition nt_str(s: list Z)(a: word): mem -> Prop :=
+  sep (array (uint 8) (len s + 1) (s ++ [| 0 |]) a)
+      (emp (~ List.In 0 s)).
 
 #[local] Hint Unfold nt_str : heapletwise_always_unfold.
 
 #[export] Instance str_cmp: fnspec :=                                           .**/
 
 uintptr_t strcmp(uintptr_t p1, uintptr_t p2) /**#
-  ghost_args := (s1 s2: list byte) (R: mem -> Prop);
+  ghost_args := (s1 s2: list Z) (R: mem -> Prop);
   requires t m := <{ * nt_str s1 p1
                      * nt_str s2 p2
                      * R }> m;
   ensures t' m' res := t' = t /\
-                       List.compare byte.compare s1 s2 = Z.compare (word.signed res) 0 /\
+                       List.compare Z.compare s1 s2 = Z.compare (word.signed res) 0 /\
                        <{ * nt_str s1 p1
                           * nt_str s2 p2
                           * R }> m' #**/                                   /**.
@@ -66,7 +58,7 @@ Derive strcmp SuchThat (fun_correct! strcmp) As strcmp_ok.                      
   | |- exec ?fs ?body ?t ?m ?l ?P =>
       lazymatch eval pattern s1, s2, p1, p2, R in P with
       | ?f s1 s2 p1 p2 R =>
-          change (exec fs body t m l ((fun (g: list byte * list byte * word * word * (mem -> Prop)) (_: Z) =>
+          change (exec fs body t m l ((fun (g: list Z * list Z * word * word * (mem -> Prop)) (_: Z) =>
      (*let '(s1, s2, p1, p2, R) := g in f s1 s2 p1 p2 R) (s1, s2, p1, p2, R) (len s1)))*)
           let (g, R) := g in
           let (g, p2) := g in
@@ -82,83 +74,33 @@ Derive strcmp SuchThat (fun_correct! strcmp) As strcmp_ok.                      
   start_loop_body.
   steps.
 
-unfold char in *.
-
   .**/
-
-
   c1 = load8(p1);                                                          /**.
+  (* TODO: how to simplify (l[0] :: l[1:]) back into l?
+     Or more also/more generally: (l[i:] ++ l[:i]) back into l?
 
-(*
-caller: array of char
-callee: expects uint8, returns same uint8
-Q: should the fact that we called a uint8 callee cast our symbolic state to uint8?
-A: not really, at least here...
+     OR could say
+     * on operations that don't modify memory: use m'=m -> no merging back is needed
+     * on opeartions taht modify memory, typically the list will change, so no
+       opportunity for this kind of simplifications *)
+  .**/
+  c2 = load8(p2);                                                          /**.
 
-maybe we need "polymorphic load"?
-or a load that doesn't cast/affect current state?
-ie a cast-callee-state load and a don't-cast_callee-state load?
-not only for loads but for any calls?
+  replace ((s2 ++ [|0|])[0] :: (s2 ++ [|0|])[1:]) with (s2 ++ [|0|]) in *.
+  2: {
+    destruct s2.
+    - bottom_up_simpl_in_goal. reflexivity.
+    - try bottom_up_simpl_in_goal. (* TODO this should simplify but doesn't *) admit.
+  }
+  replace ((s1 ++ [|0|])[0] :: (s1 ++ [|0|])[1:]) with (s1 ++ [|0|]) in * by admit.
 
+  unfold ready.
 
-caller: P
-callee pre: casted P', post Q'
-caller: cast Q' back to Q or leave as Q'??, aka use callee format or keep caller format?
-
-
-array of bytes
-read/write uint8(Z)
--> want back array of bytes (keep caller format)
-
-array of bytes
-read as packet
--> want packet (adopt callee format)
-
-packet
-memcpy bytes of packet
--> still want packet (keep caller format)
-
-
-Possible criteria:
-* If part of a struct or array, cast back to original type, otherwise keep type of callee
-  (that's a caller-based criterion)
-* Caller's postcondition says m'=m (in which case caller context is not updated)
-  or re-lists explicitly all clauses in post (in which case caller context is updated)
-  Doesn't work for functions that update memory but should cast back to caller's format
-  afterwards (though can this be automated?)
-
-Interesting case:
-
-
-immediate sol: use uint 8
-
-
-2: {
-
-unfold don't_know_how_to_prove.
-
- eapply contiguous_implies_anyval_of_fillable.
-                            [ eauto with contiguous
-                            | eauto with fillable] ];
-
-
-                    solve [ eapply contiguous_implies_anyval_of_fillable;
-                            [ eauto with contiguous
-                            | eauto with fillable] ];
-
-
-unfold char.
-
-step.
-
-
-
-reflexivity.
-
-.**/
-
-
-*)
+  lazymatch goal with
+  (* from hypothesis of do-while lemma: *)
+  | |- exec _ _ ?t ?m ?l (fun t' m' l' =>
+     exists b, dexpr_bool3 _ _ ?condEvar _ _ _ _) => idtac condEvar
+  end.
 
 Abort.
 
